working on HyGlobalTrans + build files.

sketch/HyGlobalTrans.v
@@ -11,29 +11,347 @@ Require Import ExtLib.Structures.Functor.
 Existing Instance Applicative_Fun.
 Existing Instance Functor_Fun.
 
-Definition tlaVar := string.
+Section localized.
+  Variable tlaState : Type.
 
-Definition tlaState := tlaVar -> R.
+  Definition StateVal (T : Type) : Type :=
+    tlaState -> T.
+  Definition DActionVal (T : Type) : Type :=
+    tlaState -> tlaState -> T.
+  Definition ActionVal (T : Type) : Type :=
+    tlaState -> @Step tlaState -> T.
+  Definition TraceVal (T : Type) := trace tlaState -> T.
 
-Definition StateProp := tlaState -> Prop.
+  Definition StateProp := StateVal Prop.
 
-Definition DActionProp := tlaState -> tlaState -> Prop.
-Definition CActionProp := forall (t : R) (f : R -> tlaState), Prop.
+  Definition DActionProp := DActionVal Prop.
+  Definition CActionProp := forall (t : R) (f : R -> tlaState), Prop.
 
-Definition ActionProp := tlaState -> @Step tlaState -> Prop.
+  Definition ActionProp := ActionVal Prop.
 
-Definition TraceProp := trace tlaState -> Prop.
+  Definition TraceProp := TraceVal Prop.
 
-Instance ILogicOps_StateProp : ILogicOps StateProp := @ILInsts.ILFun_Ops _ _ _.
-Instance ILogicOps_ActionProp : ILogicOps ActionProp := @ILInsts.ILFun_Ops _ _ _.
-Instance ILogicOps_DActionProp : ILogicOps DActionProp := @ILInsts.ILFun_Ops _ _ _.
-Instance ILogicOps_CActionProp : ILogicOps CActionProp := @ILInsts.ILFun_Ops _ _ _.
-Instance ILogicOps_TraceProp : ILogicOps TraceProp := @ILInsts.ILFun_Ops _ _ _.
-Instance ILogic_StateProp : ILogic StateProp. Admitted.
-Instance ILogic_ActionProp : ILogic ActionProp. Admitted.
-Instance ILogic_DActionProp : ILogic DActionProp. Admitted.
-Instance ILogic_CActionProp : ILogic CActionProp. Admitted.
-Instance ILogic_TraceProp : ILogic TraceProp. Admitted.
+  Global Instance ILogicOps_StateProp : ILogicOps StateProp := @ILInsts.ILFun_Ops _ _ _.
+  Global Instance ILogicOps_ActionProp : ILogicOps ActionProp := @ILInsts.ILFun_Ops _ _ _.
+  Global Instance ILogicOps_DActionProp : ILogicOps DActionProp := @ILInsts.ILFun_Ops _ _ _.
+  Global Instance ILogicOps_CActionProp : ILogicOps CActionProp := @ILInsts.ILFun_Ops _ _ _.
+  Global Instance ILogicOps_TraceProp : ILogicOps TraceProp := @ILInsts.ILFun_Ops _ _ _.
+  Global Instance ILogic_StateProp : ILogic StateProp. Admitted.
+  Global Instance ILogic_ActionProp : ILogic ActionProp. Admitted.
+  Global Instance ILogic_DActionProp : ILogic DActionProp. Admitted.
+  Global Instance ILogic_CActionProp : ILogic CActionProp. Admitted.
+  Global Instance ILogic_TraceProp : ILogic TraceProp. Admitted.
+
+  (* These are the "obvious" definitions, needed to help Coq *)
+  Global Instance Applicative_Action
+  : Applicative ActionVal :=
+  { pure := fun _ x => fun _ _ => x
+  ; ap := fun _ _ f x => fun st st' => (f st st') (x st st')
+  }.
+
+  Global Instance Functor_Action
+  : Functor ActionVal :=
+  { fmap := fun _ _ f x => ap (pure f) x }.
+
+  Global Instance Applicative_DAction
+  : Applicative DActionVal :=
+  { pure := fun _ x => fun _ _ => x
+  ; ap := fun _ _ f x => fun st st' => (f st st') (x st st')
+  }.
+
+  Global Instance Functor_DAction
+  : Functor DActionVal :=
+  { fmap := fun _ _ f x => ap (pure f) x }.
+
+  Global Instance Applicative_State
+  : Applicative StateVal :=
+  { pure := fun _ x => fun _ => x
+  ; ap := fun _ _ f x => fun st => (f st) (x st)
+  }.
+
+  Global Instance Functor_State
+  : Functor StateVal :=
+  { fmap := fun _ _ f x => ap (pure f) x }.
+
+
+  Definition now : StateProp -> TraceProp :=
+    fun P tr => P (HyStreamTrans.hd tr).
+
+  Definition next : StateProp -> TraceProp :=
+    fun P tr => P (HyStreamTrans.hd (HyStreamTrans.tl tr)).
+
+  Definition always (P : TraceProp) : TraceProp :=
+    fun s =>
+      forall s', HyStreamTrans.skips_to s s' -> P s'.
+
+  Definition eventually (P : TraceProp) : TraceProp :=
+    fun s =>
+      exists s', HyStreamTrans.skips_to s s' /\ P s'.
+
+  Definition discretely (P : DActionProp) : ActionProp :=
+    fun start step =>
+      match step with
+      | DiscreteTo st' =>
+        P start st'
+      | _ => False
+      end.
+
+  Definition continuously (P : CActionProp) : ActionProp :=
+    fun start step =>
+      match step with
+      | ContinuousBy r f => P r f
+      | _ => False
+      end.
+
+  Definition stutter {T} (f : tlaState -> T) : DActionProp :=
+    fun st st' => f st = f st'.
+
+  Definition starts (P : ActionProp) : TraceProp :=
+    fun tr =>
+      P (HyStreamTrans.hd tr) (firstStep tr).
+
+(*
+  Definition get {T} : tlaVar T -> tlaState -> T := record_get.
+
+  Definition pre {T} (v : tlaVar T) : DActionVal T :=
+    fun st _ => get v st.
+
+  Definition post {T} (v : tlaVar T) : DActionVal T :=
+    fun _ st' => get v st'.
+*)
+
+  Definition lift {X T U} (f : T -> U)
+    : (X -> T) -> X -> U.
+    refine (ap (pure f)).
+  Defined.
+
+  Definition lift2 {X T U V} (f : T -> U -> V)
+    : (X -> T) -> (X -> U) -> X -> V.
+    refine (fun a b => ap (ap (pure f) a) b).
+  Defined.
+
+
+  Definition through (P : TraceProp) : TraceProp :=
+    fun tr =>
+      match firstStep tr with
+      | ContinuousBy r f =>
+        forall r', (0 < r' <= r)%R ->
+                   forall tr', after_time r' 0 tr tr' ->
+                               P tr'
+      | DiscreteTo _ =>
+        forall tr', after_time 0 1 tr tr' ->
+                    P tr'
+      end.
+
+  Lemma always_skips_to : forall P t1 t2,
+      skips_to t1 t2 ->
+      always P t1 -> always P t2.
+  Proof.
+    unfold always. intros.
+    eapply H0. etransitivity; eauto.
+  Qed.
+
+  (** This is induction over the phase changes **)
+  Lemma dind_lem : forall G P,
+      G |-- P -->> always (P -->> through P) -->> always P.
+  Proof.
+    intros. red. red. Transparent ILInsts.ILFun_Ops.
+    red.
+    intros. red. simpl. red.
+    intros. clear H. clear G. revert H0 H1.
+    induction H2; simpl.
+    { (* Now *)
+      intros. assumption. }
+    { (* AfterD *)
+      intros.
+      eapply IHskips_to.
+      { red in H1.
+        specialize (H1 _ (ST_Now _) H0).
+        eapply H1. admit. }
+      { eapply always_skips_to. 2: eapply H1.
+        constructor. reflexivity. } }
+    { (* AfterC *)
+      intros.
+      eapply IHskips_to.
+      { red in H1.
+        specialize (H1 _ (ST_Now _) H0).
+        eapply H1.
+        instantiate (1:=t).
+        { admit. }
+        { admit. } }
+      { eapply always_skips_to. 2: eassumption.
+        constructor. reflexivity. } }
+    { (* WithinC *)
+      intros.
+      specialize (H1 _ (ST_Now _) H0).
+      red in H1. simpl in H1.
+      eapply H1 with (r' := r); clear H1.
+      { admit. }
+      { eapply WithinC. admit. } }
+  Qed.
+
+  Lemma always_and : forall P Q,
+      always P //\\ always Q -|- always (P //\\ Q).
+  Proof.
+    intros. split.
+    { red. red. simpl. unfold always. intuition. }
+    { red. red. simpl. unfold always. intuition;
+                                      edestruct H; eauto. }
+  Qed.
+
+  Lemma uncurry : forall P Q R,
+      (P //\\ Q) -->> R -|- P -->> Q -->> R.
+  Proof. compute. tauto. Qed.
+
+  Lemma always_impl : forall P Q,
+      |-- P -->> Q ->
+      |-- always P -->> always Q.
+  Proof. compute. intuition. Qed.
+
+  Theorem hybrid_induction
+    : forall G P T,
+      G |-- always T ->
+      G |-- P ->
+      G |-- always (P -->> T -->> through P) ->
+      G |-- always P.
+  Proof.
+    intros G P T.
+    generalize (dind_lem G P).
+    unfold lentails, ILogicOps_TraceProp. simpl.
+    intros.
+    eapply H; eauto.
+    specialize (H2 _ H3).
+    specialize (H0 _ H3).
+    revert H2. revert H0.
+    clear. revert t.
+    cut (|-- always T -->> always (P -->> T -->> through P) -->> always (P -->> through P)).
+    { intros. eapply H. exact I. auto. auto. }
+    { rewrite <- uncurry.
+      rewrite always_and.
+      eapply always_impl.
+      compute; tauto. }
+  Qed.
+
+  Lemma now_entails : forall (A B : StateProp),
+      A |-- B ->
+      now A |-- now B.
+  Proof.
+    unfold now. simpl. auto.
+  Qed.
+
+  Lemma always_tauto
+    : forall G P, |-- P -> G |-- always P.
+  Proof.
+    compute; intuition.
+  Qed.
+
+  Lemma now_starts_discretely_and : forall P Q,
+      now P //\\ starts (discretely Q) -|- starts (discretely (fun st st' => P st /\ Q st st')).
+  Proof.
+    intros. split.
+    { red; simpl. destruct t.
+      unfold starts, discretely; destruct c; simpl; tauto. }
+    { red; simpl. destruct t.
+      unfold starts, discretely; destruct c; simpl; tauto. }
+  Qed.
+
+  Lemma starts_next_impl : forall (P : DActionProp) (Q : StateProp),
+      starts (discretely (fun st st' => P st st' -> Q st')) |-- starts (discretely P) -->> next Q.
+  Proof.
+    intros.
+    { red; simpl. destruct t.
+      unfold starts, discretely; destruct c; simpl. tauto.
+      tauto. }
+  Qed.
+
+  Axiom R0_lt_R0_False : (0 < 0)%R -> False.
+  Axiom R0_gt_R0_False : (0 > 0)%R -> False.
+
+  Ltac Rarith :=
+    repeat match goal with
+           | H : (_ < _ <= _)%R |- _ => destruct H
+           | H : (_ < _ < _)%R |- _ => destruct H
+           end ;
+    solve [ eauto using R0_lt_R0_False, R0_gt_R0_False ].
+
+  Lemma starts_discretely_through : forall (P : DActionProp) (Q : StateProp),
+      (forall st, P st |-- Q) ->
+      |-- starts (discretely P) -->> through (now Q).
+  Proof.
+    intros. unfold starts, discretely, through.
+    red. simpl. intros. destruct t; simpl in *.
+    destruct c; simpl in *.
+    - exfalso; assumption.
+    - intros.
+      inversion H2; clear H2; subst.
+      { eapply after_time_now in H8. subst.
+        unfold now. simpl. eauto. }
+      { exfalso; clear - H9. Rarith. }
+  Qed.
+
+  Definition before (P : StateProp) : ActionProp :=
+    fun st _ => P st.
+
+
+
+  Definition enabled (ap : ActionProp) : StateProp :=
+    Exists st', fun st => ap st st'.
+
+  Fixpoint AnyOf {L} {LL : ILogicOps L} (ls : list L) : L :=
+    match ls with
+    | nil => lfalse
+    | cons l ls => l \\// AnyOf ls
+    end.
+
+  Fixpoint AllOf {L} {LL : ILogicOps L} (ls : list L) : L :=
+    match ls with
+    | nil => ltrue
+    | cons l ls => l //\\ AllOf ls
+    end.
+
+
+(*
+  Definition SSys (I : StateProp) (ls : list ActionProp) : TraceProp :=
+         now I
+    //\\ always (starts (     AnyOf ls
+                         \\// before (AllOf (List.map (fun x => enabled x -->> lfalse) ls))
+                         \\// discretely (stutter (fun x => x)))).
+*)
+
+  Definition Sys (I : StateProp) (d : DActionProp) : TraceProp :=
+    now I //\\ always (starts (discretely (d \\// stutter (fun x => x)))).
+
+  Definition HSys (I : StateProp) (w : CActionProp) (d : DActionProp) : TraceProp :=
+    now I //\\ always (starts (continuously w \\// discretely (d \\// stutter (fun x => x)))).
+
+
+
+
+End localized.
+
+
+Section localized.
+  Variable tlaState : Type.
+
+  Definition StateProp := tlaState -> Prop.
+
+  Definition DActionProp := tlaState -> tlaState -> Prop.
+  Definition CActionProp := forall (t : R) (f : R -> tlaState), Prop.
+
+  Definition ActionProp := tlaState -> @Step tlaState -> Prop.
+
+  Definition TraceProp := trace tlaState -> Prop.
+
+  Instance ILogicOps_StateProp : ILogicOps StateProp := @ILInsts.ILFun_Ops _ _ _.
+  Instance ILogicOps_ActionProp : ILogicOps ActionProp := @ILInsts.ILFun_Ops _ _ _.
+  Instance ILogicOps_DActionProp : ILogicOps DActionProp := @ILInsts.ILFun_Ops _ _ _.
+  Instance ILogicOps_CActionProp : ILogicOps CActionProp := @ILInsts.ILFun_Ops _ _ _.
+  Instance ILogicOps_TraceProp : ILogicOps TraceProp := @ILInsts.ILFun_Ops _ _ _.
+  Instance ILogic_StateProp : ILogic StateProp. Admitted.
+  Instance ILogic_ActionProp : ILogic ActionProp. Admitted.
+  Instance ILogic_DActionProp : ILogic DActionProp. Admitted.
+  Instance ILogic_CActionProp : ILogic CActionProp. Admitted.
+  Instance ILogic_TraceProp : ILogic TraceProp. Admitted.
 
 (* These are the "obvious" definitions, needed to help Coq *)
 Instance Applicative_Action
